---
title: "HW5_Yi_Xiong"
author: "Yi Xiong"
date: "2021/3/4"
output: 
  pdf_document:
    toc: true
---

```{r setup, include=FALSE}
knitr::opts_chunk$set(echo = TRUE)
```

# 1.(30 points) Following the developments in modules 4.3 and 4.4, derive the expressions for ACF for:

## a.MA(1) and MA(2) models

### MA(1)

#### definition

$$
\begin{aligned}
y_{t}&=\mu +\epsilon _{t}+\theta \epsilon _{t-1}
\end{aligned}
$$

#### Autocovariance

$$
\begin{aligned}
\gamma _{0}&=E[y_{t}-E(y_{t})]^{2} \\
&=E[y_{t}-\mu] \\
&=E[\epsilon_{t}+\theta\epsilon_{t-1}]^{2} \\
&=E[\epsilon_{t}^{2}+2\theta\epsilon_{t}\epsilon_{t-1}+\theta^{2}\epsilon_{t-1}^{2}]\\
&=\theta^{2}+0+\theta^{2}\sigma^{2}\\
&=(1+\theta^{2})\sigma^{2}
\end{aligned}
$$

$$
\begin{aligned}
\gamma_{j}&=E[(y_{t}-\mu)(y_{t-j}-\mu)]\\
&=E[(\epsilon_{t}+\theta\epsilon_{t-1})(\epsilon_{t-j}+\theta\epsilon_{t-j-1})]\\
&=\left\{
	\begin{array}{ll}
		\theta E[\epsilon^{2}_{t-1}]=\sigma\theta^{2} \;\; if\; j=1 \\
		0 \;\; otherwise
	\end{array}\right.
\end{aligned}	
$$

#### Autocorrelation

$$
\begin{aligned}
\rho_{j}=\frac{\gamma_{j}}{\gamma_{0}}
=\frac{\theta\sigma^{2}}{(1+\theta^{2})\sigma^{2}}
=\left\{
	\begin{array}{ll}
	  \frac{\theta}{(1+\theta^{2})} \;\; if\; j=1 \\
	  0 \;\; if\; j\neq 1
	\end{array}\right.
\end{aligned}	
$$

### MA(2)


#### MA(q) definition

$$
\begin{aligned}
y_{t}&=\mu+\sum^{q}_{j=0}\theta_{j}\epsilon_{t-j},
\;q\geqslant 1\;and \; \theta_{0}=1
\end{aligned}	
$$

#### MA(2) definition

$$
\begin{aligned}
y_{t}&=\mu+\epsilon_{t}+\theta_{1}\epsilon_{t-1}+\theta_{2}\epsilon_{t-2}
\end{aligned}	
$$

#### Autocovariance of MA(q)

$$
\begin{aligned}
\gamma_{0}&=E(y_{t}-\mu)^{2}\\
&=[\sum^{q}_{j=0}\theta_{j}^{2}]\sigma^{2}
\end{aligned}	
$$


$$
\begin{aligned}
\gamma_{j}&=E[(y_{t}-\mu)(y_{t-j}-\mu)]\\
\gamma_{j}&=\left\{
	\begin{array}{ll}
	  (\theta_{j}+\theta_{j+1}\theta_{1}+\theta_{j+2}\theta_{2}+...+\theta_{q}
	  \theta_{q-j})\sigma^{2}\;for\;1\leqslant j\leqslant q\\
	  0 \;\; for\; j>q
	\end{array}\right.
\end{aligned}	
$$

#### Autocovariance of MA(2)

$$
\begin{aligned}
\gamma_{0}=(1+\theta^{2}_{1}+\theta^{2}_{2})\sigma^{2}\\
\gamma_{1}=(\theta_{1}+\theta_{2}\theta_{1})\sigma^{2} \\
\gamma_{2}=\theta_{2}\sigma^{2}\\
\gamma_{j}=0,\;j\geqslant3
\end{aligned}
$$

#### Autocorrelation of MA(2)

$$
\begin{aligned}
\rho_{1}=\frac{(\theta_{1}+\theta_{2}\theta_{1})\sigma^{2}}
  {(1+\theta^{2}_{1}+\theta^{2}_{2})\sigma^{2}}\\
\rho_{2}=  \frac{\theta_{2}\sigma^{2}}
  {(1+\theta^{2}_{1}+\theta^{2}_{2})\sigma^{2}}\\
\rho_{j}=0,\;j\geqslant3
\end{aligned}
$$

## b.AR(1) and AR(2) models 

### AR(1)

#### definition

$$
\begin{aligned}
y_{t}=c+\phi y_{t-1}+\epsilon_{t}
\end{aligned}	
$$

#### Autocovariance  
  
##### When $|\phi|$ < 1, y~t~ is weakly stationary and ergodic 

$$
\begin{aligned}
y_{t}-\mu&=\phi(y_{t-1}-\mu)+\epsilon_{t}\\
\\
\gamma_{0}&=E[y_{t}-\mu]^{2}\\
  &=\sigma^{2}[1+\phi^{2}+\phi^{4}+...+\phi^{2k}+...]\\
  &=\frac{\sigma^2}{1-\phi^{2}}
\end{aligned}	
$$

$$
\begin{aligned}
\gamma_{j}&=E[(y_{t}-\mu)(y_{t-j}-\mu)]\\
  &=\sigma^{2}[\phi^{j}+\phi^{j+2}+\phi^{j+4}+...]\\
  &=\sigma^{2}\phi^{j}[1+\phi^{2}+\phi^{4}+...]\\
  &=\sigma^{2}\frac{\phi^{j}}{1-\phi^{2}}
\end{aligned}	
$$


#### Autocorrelation

$$
\begin{aligned}
\rho_{j}=\frac{\gamma_{j}}{\gamma_{0}}=\phi^{j}
\end{aligned}	
$$


$$
\begin{aligned}
\end{aligned}	
$$

### AR(2)

#### definition

$$
\begin{aligned}
y_{t}=c+\phi_{1}y_{t-1}+\phi_{2}y_{t-2}+\epsilon_{t}
\end{aligned}	
$$

##### For stationarity:

$$
\begin{aligned}
&\lambda^{2}-\phi_{1}\lambda-\phi_{2}=0\\
&\lambda=\frac{\phi_{1}\pm\sqrt{\phi^{2}_{1}+4\phi2}}{2}\\
&|\lambda|<1
\end{aligned}	
$$

#### Autocovariance

$$
\begin{aligned}
y_{t}-\mu=\phi_{1}(y_{t-1}-\mu)+\phi_{2}(y_{t-2}-\mu)+\epsilon_{t}
\end{aligned}	
$$

$$
\begin{aligned}
\gamma_{0}&=E[(y_{t}-\mu)(y_{t}-\mu)]\\
  &=E[\phi_{1}(y_{t}-\mu)(y_{t-1}-\mu)]\\
    &+E[\phi_{2}(y_{t}-\mu)(y_{t-2}-\mu)]\\
    &+E[(y_{t}-\mu)\epsilon_{t}]\\
  &=\phi_{1}\gamma_{1}+\phi_{2}\gamma_{2}+\sigma^{2}
\end{aligned}	
$$

$$
\begin{aligned}
for \;j&\geqslant1\\
\\
\gamma_{j}&=E[(y_{t}-\mu)(y_{t-j}-\mu)]\\
  &=E[\phi_{1}(y_{t-1}-\mu)(y_{t-j}-\mu)]\\
    &+E[\phi_{2}(y_{t-2}-\mu)(y_{t-j}-\mu)]\\
    &+E[(y_{t-j}-\mu)\epsilon_{t}]\\
  &=\phi_{1}\gamma_{1}+\phi_{2}\gamma_{2}
\end{aligned}	
$$


#### Autocorrelation


$$
\begin{aligned}
for \;j&\geqslant1\\
\\
\rho_{j}&=\frac{\gamma_{j}}{\gamma_{0}}\\
  &=\theta_{1}\frac{\gamma_{j-1}}{\gamma_{0}}+
    \theta_{2}\frac{\gamma_{j-2}}{\gamma_{0}}\\
  &=\phi_{1}\rho_{j-1}+\phi_{2}\rho_{j-2}
\end{aligned}	
$$


$$
\begin{aligned}
\rho_{1}&=\phi_{1}\rho_{0}+\phi_{2}\rho_{-1}\\
  \rho_{1}&=\frac{\phi_{1}}{1-\phi_{2}}\\
\rho_{2}&=\phi_{1}\rho_{1}+\phi_{2}\rho_{0}\\
  &=\phi_{1}\rho_{1}+\phi_{2}
\end{aligned}	
$$


$$
\begin{aligned}
\gamma_{0}=\frac{(1-\phi_{2})\sigma^{2}}{(1+\phi_{2})
  [(1-\phi_{2})^{2}-\phi^{2}_{1}]}
\end{aligned}	
$$

#### Summary

$$
\begin{aligned}
\rho_{1}&=\frac{\phi_{1}}{1-\phi_{2}}\\
\rho_{2}&=\phi_{1}\rho_{1}+\phi_{2}\\
\rho_{j}&=\phi_{1}\rho_{j-1}+\phi_{2}\rho_{j-2} \;\; for \; j\geqslant 3
\end{aligned}	
$$

# c.ARMA(1,1) 

#### definition

$$
\begin{aligned}
y_{t}=c+\phi_{1}t_{t-1}+\epsilon_{t}+\theta_{1}\epsilon_{t-1}
\end{aligned}	
$$

#### Autocovariance

$$
\begin{aligned}
y_{t}-\mu&=\phi_{1}(y_{t-1}-\mu)+\epsilon_{t}+\theta_{1}\epsilon_{t-1}\\
\\
\gamma_{0}&=E[y_{t}-\mu]^{2}\\
&=E[\phi_{1}(y_{t-1}-\mu)+\epsilon_{t}+\phi_{1}\epsilon_{t-1}]^{2}\\
&=\phi_{1}^{2}\gamma_{0}+\sigma^{2}+\theta_{1}^{2}\sigma^{2}
  +2\phi_{1}\theta_{1}\sigma^{2}\\
\\
\gamma_{0}&=\frac{\sigma^{2}[1+2\phi_{1}\theta_{1}+\theta_{1}^{2}]}
{1-\theta_{1}^{2}}
\end{aligned}	
$$

$$
\begin{aligned}
\gamma_{1}&=E[(y_{t}-\mu)(y_{t-1}-\mu)]\\
&=E\{[\phi_{1}(y_{t-1}-\mu)+\epsilon_{t}+\phi_{1}\epsilon_{t-1}]
[y_{t-1}-\mu]\}\\
&=\phi_{1}\gamma_{0}+\theta_{1}\sigma^{2}
\end{aligned}	
$$

$$
\begin{aligned}
for \;j&\geqslant 2\\
\\
\gamma_{j}&=E[(y_{t}-\mu)(y_{t-j}-\mu)]\\
&=E\{[\phi_{1}(y_{t-1}-\mu)+\epsilon_{t}+\phi_{1}\epsilon_{t-1}]
[y_{t-j}-\mu]\}\\
&=\phi_{1}E[(y_{t-1}-\mu)(y_{t-j}-\mu)]\\
&=\phi_{1}\gamma_{j-1}
\end{aligned}	
$$

#### Autocorrelation

$$
\begin{aligned}
\gamma_{0}=\frac{\sigma^{2}[1+2\phi_{1}\theta_{1}+\theta_{1}^{2}]}
  {1-\phi_{1}^{2}}\\
\gamma_{1}=\phi_{1}\gamma_{0}+\theta_{1}\sigma^{2}\\
\gamma_{j}=\phi_{1}\gamma_{j-1} \;\; for \;j \geqslant 2\\
\rho_{1}=\frac{\gamma_{1}}{\gamma_{0}}\\
\rho_{j}=\frac{\gamma_{j}}{\gamma_{0}}
\end{aligned}	
$$
