---
title: "MID-TERM EXAM - 2"
author: "Yi Xiong"
date: "2021/4/14"
output: 
  pdf_document:
    toc: true
---

```{r setup, include=FALSE}
knitr::opts_chunk$set(echo = TRUE)
```

# 1.(20+20 pts) Apply the method of module 7.2 for estimating the parameters a and b in the model 
  
  
from a set of m samples $(y_i , x_i ),\; 1 \leqslant  i \leqslant m.$  
  
  
## A) $y = a + e^{-bx}$  

define a linear relation

$$
\begin{aligned}
y_i=a+bx_i
\end{aligned}	
$$
by the Least Squares method we estimate the parameters a and b 

$$
\begin{aligned}
\hat{b}&=\frac{\bar{xy}-\bar{x}\bar{y}}{\bar{x^2}-(\bar{x})^2} \\
  &=\frac{m\sum_{i=1}^{m}x_iy_i-(\sum_{i=1}^{m}x_i)(\sum_{i=1}^{m}y_i)}
    {m(\sum_{i=1}^{m}x_i^2)-(\sum_{i=1}^{m}x_i)^2} \\
\\    
\hat{a}&=\frac{1}{m}\left [ \sum_{i=1}^{m}y_i-\hat{b}\sum_{i=1}^{m}x_i\right ]\\
&=\bar{y}-\hat{b}\bar{x}
\end{aligned}	
$$

convert

$$
\begin{aligned}
y &= a + e^{-bx}\\
\ln(y)&=\ln(a)-bx
\end{aligned}	
$$

let ${y_i}'=\ln(y_i)$ ${a}'=\ln(a)$ ${b}'=-b$

$$
\begin{aligned}
{y_i}'={a}'+{b}'x_i
\end{aligned}	
$$

$$
\begin{aligned}
\hat{{b}'}&=\frac{\bar{x\ln(y)}-\bar{x}\bar{ln(y)}}{\bar{x^2}-(\bar{x})^2} \\
  &=\frac{m\sum_{i=1}^{m}x_i \ln(y_i)-(\sum_{i=1}^{m}x_i)(\sum_{i=1}^{m} \ln(y_i)}
    {m(\sum_{i=1}^{m}x_i^2)-(\sum_{i=1}^{m}x_i)^2} \\
\hat{b}&=-\hat{{b}'}\\
\\    
\hat{{a}'}&=\frac{1}{m}\left [ \sum_{i=1}^{m}\ln(y_i)-\hat{{b}}'\sum_{i=1}^{m}x_i\right ]\\
&=\bar{\ln(y)}-\hat{{b}'}\bar{x}\\
a&=e^{{a}'}\\
a&=\bar{y}e^{\hat{b}\bar{x}}\\
\end{aligned}	
$$

## B) $y = c + mx$ 

let  ${a}'=c$ ${b}'=m$

$$
\begin{aligned}
{y_i}={a}'+{b}'x_i
\end{aligned}	
$$

convert

$$
\begin{aligned}
\hat{m}&=\frac{\bar{xy}-\bar{x}\bar{y}}{\bar{x^2}-(\bar{x})^2} \\
  &=\frac{m\sum_{i=1}^{m}x_iy_i-(\sum_{i=1}^{m}x_i)(\sum_{i=1}^{m}y_i)}
    {m(\sum_{i=1}^{m}x_i^2)-(\sum_{i=1}^{m}x_i)^2} \\
\\    
\hat{c}&=\frac{1}{m}\left [ \sum_{i=1}^{m}y_i-\hat{m}\sum_{i=1}^{m}x_i\right ]\\
&=\bar{y}-\hat{m}\bar{x}
\end{aligned}	
$$